added algorithmic type judgment, changed some notation in TypeCheck.v

theories/Extraction/TypeCheck.v
@@ -33,7 +33,7 @@ Section lookup.
         let*o (existT _ B (exist _ s' _)) := lookup dec_P Γ _ x' while _ in
         pureo (existT _ {{{ B[Wk] }}} (exist _ s' _))
     }
-  | dec_P, {{{ ⋅ }}}, HG, x => inright _.
+  | dec_P, {{{ ⋅ }}}, HΓ, x => inright _.
 End lookup.
 
 Section type_check.
@@ -91,7 +91,7 @@ Section type_check.
           clear H
       | H: (let H := fixproto in
             forall (Γ : ctx P) (A : typ P),
-              (exists s : P, {{ Γ ⊢ A : Sort @ s }}) -> forall M : typ P, type_check_order M -> { {{ Γ ⊢a M ⟸ A }} } + { ~ {{ G ⊢a M ⟸ A }} })
+              (exists s : P, {{ Γ ⊢ A : Sort @ s }}) -> forall M : typ P, type_check_order M -> { {{ Γ ⊢a M ⟸ A }} } + { ~ {{ Γ ⊢a M ⟸ A }} })
         |- _ =>
           clear H
       | H: (let H := fixproto in
@@ -99,15 +99,14 @@ Section type_check.
               {{ ⊢ Γ }} ->
               forall M : typ P,
                 type_infer_order M ->
-                (* This will pose problems, we probably need an algorithmic type well-formedness check *)
-                ({ B : nf P | {{ Γ ⊢a M ⟹ B }} /\ (exists s : P, {{ Γ ⊢a ^(nf_to_exp B) ⟹ Sort@s }}) } + { forall C : nf P, ~ {{ Γ ⊢a M ⟹ C }} }))
+                ({ B : nf P | {{ Γ ⊢a M ⟹ B }} /\ {{ Γ ⊢aty ^(nf_to_exp B) }} } + { forall C : nf P, ~ {{ Γ ⊢a M ⟹ C }} }))
         |- _ =>
           clear H
       | H: (forall Γ : ctx P,
                {{ ⊢ Γ }} ->
                forall M : typ P,
                  type_infer_order M ->
-                 ({ B : nf P | {{ Γ ⊢a M ⟹ B }} /\ (exists s : P, {{ Γ ⊢a ^(nf_to_exp B) ⟹ Sort@s }}) } + { forall C : nf P, ~ {{ Γ ⊢a M ⟹ C }} }))
+                 ({ B : nf P | {{ Γ ⊢a M ⟹ B }} /\{{ Γ ⊢aty ^(nf_to_exp B) }} } + { forall C : nf P, ~ {{ Γ ⊢a M ⟹ C }} }))
         |- _ =>
           clear H
     end.
@@ -115,14 +114,12 @@ Section type_check.
   #[local]
   Ltac clear_redundant_pat :=
     repeat match goal with
-      | H: { A | {{ ^?G ⊢a ^?M ⟹ A }} /\ (exists i : nat, {{ ^?G ⊢a ^(nf_to_exp A) ⟹ Sort@i }}) }
-          , H1: {{ ^?G ⊢a ^?M ⟹ ^?B }} /\ (exists i : nat, {{ ^?G ⊢a ^(nf_to_exp ?B) ⟹ Sort@i }}) |- _ => clear H
-      | H: { i | ?A = n{{{ Sort@i }}} }
-          , H1: ?A = n{{{ Sort@?i }}} |- _ => clear H
-      | H: { B & { C | ?A = n{{{ Π B C }}} } }
-          , H1: ?A = n{{{ Π ^?B ^?C }}} |- _ => clear H
-      | H: { B & { C | ?A = n{{{ Σ B C }}} } }
-          , H1: ?A = n{{{ Σ ^?B ^?C }}} |- _ => clear H
+      | H: { A | {{ ^?Γ ⊢a ^?M ⟹ A }} /\ (exists s, {{ ^?Γ ⊢a ^(nf_to_exp A) ⟹ Sort@s }}) }
+          , H1: {{ ^?Γ ⊢a ^?M ⟹ ^?B }} /\ (exists s, {{ ^?Γ ⊢a ^(nf_to_exp ?B) ⟹ Sort@s }}) |- _ => clear H
+      | H: { s | ?A = n{{{ Sort@s }}} }
+          , H1: ?A = n{{{ Sort@?s }}} |- _ => clear H
+      | H: { B & { C | ?A = n{{{ Π ?r B C }}} } }
+          , H1: ?A = n{{{ Π ?r ^?B ^?C }}} |- _ => clear H
       end.
 
   #[local]
@@ -135,100 +132,54 @@ Section type_check.
   Ltac impl_obl_tac := clean_obl; eauto 3.
 
   #[tactic="impl_obl_tac",derive(equations=no,eliminator=no)]
-  Equations type_check G A (HA : (exists i, {{ G ⊢ A : Sort@i }})) M (H : type_check_order M) : { {{ G ⊢a M ⟸ A }} } + { ~ {{ G ⊢a M ⟸ A }} } by struct H :=
-  | G, A, HA, M, H =>
-      let*o->b (exist _ B _) := type_infer G _ M _ while _ in
-      let*b _ := subtyping_impl G (B : nf) A _ while _ in
+  Equations type_check {P : PtsSig} (dec_P : DecidableSig P) (Γ : ctx P) A (HA : (exists i, {{ Γ ⊢ A : Sort@i }})) M (H : type_check_order M) : { {{ Γ ⊢a M ⟸ A }} } + { ~ {{ Γ ⊢a M ⟸ A }} } by struct H :=
+  | dec_P, Γ, A, HA, M, H =>
+      let*o->b (exist _ B _) := type_infer dec_P Γ _ M _ while _ in
+      let*b _ := subtyping_impl dec_P Γ (B : nf P) A _ while _ in
       pureb _
-  with type_infer G (HG : {{ ⊢ G }}) M (H : type_infer_order M) : { A : nf | {{ G ⊢a M ⟹ A }} /\ (exists i, {{ G ⊢a A ⟹ Sort@i }}) } + { forall A, ~ {{ G ⊢a M ⟹ A }} } by struct H :=
-  | G, HG, M, H with M => {
-    | {{{ Sort@j }}} =>
-        pureo (exist _ n{{{ Sort@(S j) }}} _)
+  with type_infer {P : PtsSig} (dec_P : DecidableSig P) (Γ : ctx P) (HΓ : {{ ⊢ Γ }}) M (H : type_infer_order M) : { A : nf P | {{ Γ ⊢a M ⟹ A }} /\ {{ Γ ⊢aty A }} } + { forall A, ~ {{ Γ ⊢a M ⟹ A }} } by struct H :=
+  | dec_P, Γ, HΓ, M, H with M => {
+    | {{{ Sort@s }}} =>
+        (* pureo (exist _ n{{{ Sort@(S s) }}} _) *)
+        _ 
     | {{{ ℕ }}} =>
         pureo (exist _ n{{{ Sort@0 }}} _)
     | {{{ zero }}} =>
         pureo (exist _ n{{{ ℕ }}} _)
     | {{{ succ M' }}} =>
-        let*b->o _ := type_check G {{{ ℕ }}} _ M' _ while _ in
+        let*b->o _ := type_check Γ {{{ ℕ }}} _ M' _ while _ in
         pureo (exist _ n{{{ ℕ }}} _)
     | {{{ rec M' return A' | zero -> MZ | succ -> MS end }}} =>
-        let*b->o _ := type_check G {{{ ℕ }}} _ M' _ while _ in
-        let*o (exist _ UA' _) := type_infer {{{ G, ℕ }}} _ A' _ while _ in
-        let*o (exist _ i _) :=  get_level_of_type_nf UA' while _ in
-        let*b->o _ := type_check G {{{ A'[Id,,zero] }}} _ MZ _ while _ in
-        let*b->o _ := type_check {{{ G, ℕ, A' }}} {{{ A'[Wk∘Wk,,succ #1] }}} _ MS _ while _ in
-        let (A'', _) := nbe_ty_impl G {{{ A'[Id,,M'] }}} _ in
+        let*b->o _ := type_check Γ {{{ ℕ }}} _ M' _ while _ in
+        let*o (exist _ UA' _) := type_infer {{{ Γ, ℕ@s }}} _ A' _ while _ in
+        let*o (exist _ s' _) :=  get_level_of_sort_nf UA' while _ in
+        let*b->o _ := type_check Γ {{{ A'[Id,,zero] }}} _ MZ _ while _ in
+        let*b->o _ := type_check {{{ Γ, ℕ@s, A'@s' }}} {{{ A'[Wk∘Wk,,succ #1] }}} _ MS _ while _ in
+        let (A'', _) := nbe_ty_impl Γ {{{ A'[Id,,M'] }}} _ in
         pureo (exist _ A'' _)
-    | {{{ Π B C }}} =>
-        let*o (exist _ UB _) := type_infer G _ B _ while _ in
-        let*o (exist _ i _) :=  get_level_of_type_nf UB while _ in
-        let*o (exist _ UC _) := type_infer {{{ G, B }}} _ C _ while _ in
-        let*o (exist _ j _) :=  get_level_of_type_nf UC while _ in
-        pureo (exist _ n{{{ Sort@(max i j) }}} _)
-    | {{{ λ A' M' }}} =>
-        let*o (exist _ UA' _) := type_infer G _ A' _ while _ in
-        let*o (exist _ i _) :=  get_level_of_type_nf UA' while _ in
-        let*o (exist _ B' _) := type_infer {{{ G, A' }}} _ M' _ while _ in
-        let (A'', _) := nbe_ty_impl G A' _ in
-        pureo (exist _ n{{{ Π A'' B' }}} _)
+    | {{{ Π r B C }}} =>
+        let*o (exist _ UB _) := type_infer dec_P Γ _ B _ while _ in
+        let*o (exist _ s _) :=  get_level_of_sort_nf dec_P UB while _ in
+        let*o (exist _ UC _) := type_infer dec_P {{{ Γ, B@s }}} _ C _ while _ in
+        let*o (exist _ j _) :=  get_level_of_sort_nf dec_P UC while _ in
+        (* pureo (exist _ n{{{ Sort@(max i j) }}} _) *)
+        _
+    | {{{ λ r A' B' M' }}} =>
+        let*o (exist _ UA' _) := type_infer dec_P Γ _ A' _ while _ in
+        let*o (exist _ s _) :=  get_level_of_sort_nf dec_P UA' while _ in
+        let*o (exist _ B' _) := type_infer dec_P  {{{ Γ, A'@s }}} _ M' _ while _ in
+        let (A'', _) := nbe_ty_impl Γ A' _ in
+        pureo (exist _ n{{{ Π r A'' B' }}} _)
     | {{{ M' N' }}} =>
-        let*o (exist _ C _) := type_infer G _ M' _ while _ in
-        let*o (existT _ A (exist _ B _)) := get_subterms_of_pi_nf C while _ in
-        let*b->o _ := type_check G (A : nf) _ N' _ while _ in
-        let (B', _) := nbe_ty_impl G {{{ ^(B : nf)[Id,,N'] }}} _ in
+        let*o (exist _ C _) := type_infer dec_P Γ _ M' _ while _ in
+        let*o (existT _ s1 (existT _ s2 (existT _ s3 (existT _ r (existT _ A (exist _ B _)))))) :=
+          get_subterms_of_pi_nf dec_P C while _ in
+        let*b->o _ := type_check dec_P Γ (A : nf P) _ N' _ while _ in
+        let (B', _) := nbe_ty_impl Γ {{{ ^(B : nf P)[Id,,N'] }}} _ in
         pureo (exist _ B' _)
-    | {{{ Σ B C }}} =>
-        let*o (exist _ UB _) := type_infer G _ B _ while _ in
-        let*o (exist _ i _) :=  get_level_of_type_nf UB while _ in
-        let*o (exist _ UC _) := type_infer {{{ G, B }}} _ C _ while _ in
-        let*o (exist _ j _) :=  get_level_of_type_nf UC while _ in
-        pureo (exist _ n{{{ Sort@(max i j) }}} _)
-    | {{{ ⟨ M1' : A' ; M2' : B' ⟩ }}} =>
-        let*o (exist _ UA' _) := type_infer G _ A' _ while _ in
-        let*o (exist _ i _) :=  get_level_of_type_nf UA' while _ in
-        let*o (exist _ UB' _) := type_infer {{{ G , A' }}} _ B' _ while _ in
-        let*o (exist _ j _) :=  get_level_of_type_nf UB' while _ in
-        let*b->o _ := type_check G A' _ M1' _ while _ in
-        let*b->o _ := type_check G {{{ B'[Id,,M1'] }}} _ M2' _ while _ in
-        let (A'', _) := nbe_ty_impl G A' _ in
-        let (B'', _) := nbe_ty_impl {{{ G , A' }}} B' _ in
-        pureo (exist _ n{{{ Σ A'' B'' }}} _)
-    | {{{ fst M' }}} =>
-        let*o (exist _ C _) := type_infer G _ M' _ while _ in
-        let*o (existT _ A' (exist _ B _)) := get_subterms_of_sigma_nf C while _ in
-        pureo (exist _ A' _)
-    | {{{ snd M' }}} =>
-        let*o (exist _ C _) := type_infer G _ M' _ while _ in
-        let*o (existT _ A' (exist _ B _)) := get_subterms_of_sigma_nf C while _ in
-        let (B', _) := nbe_ty_impl G {{{ B[Id,,fst M'] }}} _ in
-        pureo (exist _ B' _)
-    | {{{ Eq A' M1' M2' }}} =>
-        let*o (exist _ UA' _) := type_infer G _ A' _ while _ in
-        let*o (exist _ i _) :=  get_level_of_type_nf UA' while _ in
-        let*b->o _ := type_check G A' _ M1' _ while _ in
-        let*b->o _ := type_check G A' _ M2' _ while _ in
-        pureo (exist _ n{{{ Sort@i }}} _)
-    | {{{ refl A' M' }}} =>
-        let*o (exist _ UA' _) := type_infer G _ A' _ while _ in
-        let*o (exist _ i _) :=  get_level_of_type_nf UA' while _ in
-        let*b->o _ := type_check G A' _ M' _ while _ in
-        let (A'', _) := nbe_ty_impl G A' _ in
-        let (M'', _) := nbe_impl G M' A' _ in
-        pureo (exist _ n{{{ Eq A'' M'' M'' }}} _)
-    | {{{ eqrec N' as Eq A' M1' M2' return B' | refl -> BR' end }}} =>
-        let*o (exist _ UA' _) := type_infer G _ A' _ while _ in
-        let*o (exist _ i _) :=  get_level_of_type_nf UA' while _ in
-        let*b->o _ := type_check G A' _ M1' _ while _ in
-        let*b->o _ := type_check G A' _ M2' _ while _ in
-        let*o (exist _ UB' _) := type_infer {{{ G, A', A'[Wk], Eq A'[Wk∘Wk] #1 #0 }}} _ B' _ while _ in
-        let*o (exist _ j _) :=  get_level_of_type_nf UB' while _ in
-        let*b->o _ := type_check {{{ G, A' }}} {{{ B'[Id,,#0,,refl A'[Wk] #0] }}} _ BR' _ while _ in
-        let*b->o _ := type_check G {{{ Eq A' M1' M2' }}} _ N' _ while _ in
-        let (B'', _) := nbe_ty_impl G {{{ B'[Id,,M1',,M2',,N'] }}} _ in
-        pureo (exist _ B'' _)
     | {{{ #x }}} =>
-        let*o (exist _ A _) := lookup G _ x while _ in
-        let (A', _) := nbe_ty_impl G A _ in
+        let*o (existT _ A (exist _ s' _)) := lookup dec_P Γ _ x while _ in
+        let (A', _) := nbe_ty_impl Γ A _ in
         pureo (exist _ A' _)
     | _ => inright _
     }
@@ -252,11 +203,11 @@ Section type_check.
   #[local]
   Ltac impl_wf_context_obl_tac :=
     lazymatch goal with
-      | |- {{ ⊢ ^?G, ^?A }} =>
+      | |- {{ ⊢ ^?Γ, ^?A }} =>
           gen_presups;
-          assert {{ ⊢ G }} by mauto 2;
-          unshelve (eassert {{ G ⊢ A : ^n{{{ Sort@_ }}} }}; solve [mauto 2 using alg_type_infer_sound]); solve [constructor]
-      | |- {{ ⊢ ^?G }} => gen_presups; mauto 2
+          assert {{ ⊢ Γ }} by mauto 2;
+          unshelve (eassert {{ Γ ⊢ A : ^n{{{ Sort@_ }}} }}; solve [mauto 2 using alg_type_infer_sound]); solve [constructor]
+      | |- {{ ⊢ ^?Γ }} => gen_presups; mauto 2
       end.
 
   #[local]
@@ -272,27 +223,27 @@ Section type_check.
   #[local]
   Ltac resolve_alg_sound :=
     repeat match goal with
-      | H: {{ ^?G ⊢a ^?M ⟹ ^?A }} |- _ => assert {{ G ⊢ M : A }} by eauto 2 using alg_type_infer_sound; fail_if_dup
-      | H: {{ ^?G ⊢a ^?M ⟸ ^?A }} |- _ => assert {{ G ⊢ M : A }} by eauto 2 using alg_type_check_sound; fail_if_dup
+      | H: {{ ^?Γ ⊢a ^?M ⟹ ^?A }} |- _ => assert {{ Γ ⊢ M : A }} by eauto 2 using alg_type_infer_sound; fail_if_dup
+      | H: {{ ^?Γ ⊢a ^?M ⟸ ^?A }} |- _ => assert {{ Γ ⊢ M : A }} by eauto 2 using alg_type_check_sound; fail_if_dup
       end.
 
   #[local]
   Ltac simplify_nbe_order :=
     lazymatch goal with
-    | |- nbe_ty_order ?G ?A => enough (exists i, {{ G ⊢ A : ^(nf_to_exp (nf_typ i)) }}) as [? [? []]%soundness_ty] by eauto 3 using nbe_ty_order_sound
-    | |- nbe_order ?G ?M ?A => enough ({{ G ⊢ M : A }}) as [? []]%soundness by eauto 3 using nbe_order_sound
+    | |- nbe_ty_order ?Γ ?A => enough (exists i, {{ Γ ⊢ A : ^(nf_to_exp (nf_typ i)) }}) as [? [? []]%soundness_ty] by eauto 3 using nbe_ty_order_sound
+    | |- nbe_order ?Γ ?M ?A => enough ({{ Γ ⊢ M : A }}) as [? []]%soundness by eauto 3 using nbe_order_sound
     end.
 
   #[local]
   Ltac impl_nbe_order_obl_tac :=
     lazymatch goal with
-    | |- nbe_ty_order ?G ?A =>
+    | |- nbe_ty_order ?Γ ?A =>
         gen_presups;
         resolve_alg_sound;
         simplify_nbe_order;
         unshelve (eexists; solve [eauto 2]);
         solve [constructor]
-    | |- nbe_order ?G ?M ?A =>
+    | |- nbe_order ?Γ ?M ?A =>
         gen_presups;
         resolve_alg_sound;
         simplify_nbe_order;
@@ -302,16 +253,16 @@ Section type_check.
   #[local]
   Ltac impl_subtyping_order_obl_tac :=
     match goal with
-    | |- subtyping_order ?G ?B ?A =>
+    | |- subtyping_order ?Γ ?B ?A =>
         gen_presups;
         resolve_alg_sound;
         econstructor;
         lazymatch goal with
-        | |- nbe_ty_order ?G ?A =>
+        | |- nbe_ty_order ?Γ ?A =>
             simplify_nbe_order;
             unshelve (eexists; solve [eauto 2]);
             solve [constructor]
-        | |- nbe_order ?G ?M ?A =>
+        | |- nbe_order ?Γ ?M ?A =>
             simplify_nbe_order;
             solve [eauto 2]
         end
@@ -320,8 +271,8 @@ Section type_check.
   #[local]
   Ltac impl_exist_lvl_wf_exp_obl_tac :=
     match goal with
-    | |- exists i, {{ ^?G ⊢ ^?A : Sort@i }} => enough (exists i, {{ G ⊢ A : ^(nf_to_exp (nf_typ i)) }}) by eauto 2
-    | |- exists i, {{ ^?G ⊢ ^?A : ^(nf_to_exp (nf_typ i)) }} => idtac
+    | |- exists i, {{ ^?Γ ⊢ ^?A : Sort@i }} => enough (exists i, {{ Γ ⊢ A : ^(nf_to_exp (nf_typ i)) }}) by eauto 2
+    | |- exists i, {{ ^?Γ ⊢ ^?A : ^(nf_to_exp (nf_typ i)) }} => idtac
     end;
     autoinjections;
     progressive_inversion;
@@ -352,117 +303,117 @@ Section type_check.
     mautosolve 3.
   Qed.
 
-  Next Obligation. (* exists j, {{ G ⊢ A'[Id,,zero] : Sort@j }} *)
+  Next Obligation. (* exists j, {{ Γ ⊢ A'[Id,,zero] : Sort@j }} *)
     eexists.
-    assert {{ ⊢ G, ℕ }} by mauto 3.
+    assert {{ ⊢ Γ, ℕ }} by mauto 3.
     resolve_alg_sound.
     mauto 3.
   Qed.
 
-  Next Obligation. (* exists j, {{ G, ℕ, A' ⊢ A'[Wk∘Wk,,succ #1] : Sort@i }} *)
+  Next Obligation. (* exists j, {{ Γ, ℕ, A' ⊢ A'[Wk∘Wk,,succ #1] : Sort@i }} *)
     eexists.
-    assert {{ ⊢ G, ℕ }} by mauto 3.
+    assert {{ ⊢ Γ, ℕ }} by mauto 3.
     resolve_alg_sound.
     mauto 3.
   Qed.
 
-  Next Obligation. (* nbe_ty_order G {{{ A'[Id,,M'] }}} *)
+  Next Obligation. (* nbe_ty_order Γ {{{ A'[Id,,M'] }}} *)
     simplify_nbe_order.
     eexists.
-    assert {{ G ⊢ ℕ : Sort@0 }} by mauto 2.
-    assert {{ ⊢ G, ℕ }} by mauto 2.
+    assert {{ Γ ⊢ ℕ : Sort@0 }} by mauto 2.
+    assert {{ ⊢ Γ, ℕ }} by mauto 2.
     resolve_alg_sound.
     mauto 3.
   Qed.
 
-  Next Obligation. (* {{ G ⊢a rec M' return A' | zero -> MZ | succ -> MS end ⟹ A'' }} /\ (exists j, {{ G ⊢a A'' ⟹ Sort@j }}) *)
+  Next Obligation. (* {{ Γ ⊢a rec M' return A' | zero -> MZ | succ -> MS end ⟹ A'' }} /\ (exists j, {{ Γ ⊢a A'' ⟹ Sort@j }}) *)
     split; [mautosolve 3 |].
-    assert {{ G ⊢ ℕ : Sort@0 }} by mauto 2.
-    assert {{ ⊢ G, ℕ }} by mauto 2.
+    assert {{ Γ ⊢ ℕ : Sort@0 }} by mauto 2.
+    assert {{ ⊢ Γ, ℕ }} by mauto 2.
     resolve_alg_sound.
-    assert {{ G ⊢ A'[Id,,M'] : Sort@i }} by mauto 3.
-    assert {{ G ⊢ A'[Id,,M'] ≈ A'' : Sort@i }} by eauto 2 using soundness_ty'.
+    assert {{ Γ ⊢ A'[Id,,M'] : Sort@i }} by mauto 3.
+    assert {{ Γ ⊢ A'[Id,,M'] ≈ A'' : Sort@i }} by eauto 2 using soundness_ty'.
     assert (user_exp A'') by trivial using user_exp_nf.
-    assert (exists j, {{ G ⊢a A'' ⟹ Sort@j }} /\ j <= i) as [? []] by (gen_presups; mauto 3).
+    assert (exists j, {{ Γ ⊢a A'' ⟹ Sort@j }} /\ j <= i) as [? []] by (gen_presups; mauto 3).
     eexists; eauto 2.
   Qed.
 
-  Next Obligation. (* {{ G ⊢a λ A' M' ⟹ Π A'' B' }} /\ (exists j, {{ G ⊢a Π A'' B' ⟹ Sort@j }}) *)
+  Next Obligation. (* {{ Γ ⊢a λ A' M' ⟹ Π A'' B' }} /\ (exists j, {{ Γ ⊢a Π A'' B' ⟹ Sort@j }}) *)
     split; [mautosolve 3 |].
     resolve_alg_sound.
-    assert {{ ⊢ G, A' }} by mauto 2.
-    assert {{ G ⊢ A' ≈ A'' : Sort@i }} by eauto 2 using soundness_ty'.
-    assert {{ G ⊢ A'' : Sort@i }} by (gen_presups; mauto 2).
-    assert {{ ⊢ G, ^(A'' : exp) }} by mauto 2.
+    assert {{ ⊢ Γ, A' }} by mauto 2.
+    assert {{ Γ ⊢ A' ≈ A'' : Sort@i }} by eauto 2 using soundness_ty'.
+    assert {{ Γ ⊢ A'' : Sort@i }} by (gen_presups; mauto 2).
+    assert {{ ⊢ Γ, ^(A'' : exp) }} by mauto 2.
     resolve_alg_sound.
-    assert {{ ⊢ G, A' ≈ G, ^(A'' : exp) }} by mauto 3.
-    eassert {{ G, ^(A'' : exp) ⊢ B' : Sort@_ }} by mauto 2.
+    assert {{ ⊢ Γ, A' ≈ Γ, ^(A'' : exp) }} by mauto 3.
+    eassert {{ Γ, ^(A'' : exp) ⊢ B' : Sort@_ }} by mauto 2.
     assert (user_exp A'') by trivial using user_exp_nf.
-    assert (exists j, {{ G ⊢a A'' ⟹ Sort@j }} /\ j <= i) as [? []] by (gen_presups; mauto 2).
+    assert (exists j, {{ Γ ⊢a A'' ⟹ Sort@j }} /\ j <= i) as [? []] by (gen_presups; mauto 2).
     assert (user_exp B') by trivial using user_exp_nf.
-    eassert (exists k, {{ G, ^(A'' : exp) ⊢a B' ⟹ Sort@k }} /\ k <= H1) as [? []] by (gen_presups; mauto 2).
+    eassert (exists k, {{ Γ, ^(A'' : exp) ⊢a B' ⟹ Sort@k }} /\ k <= H1) as [? []] by (gen_presups; mauto 2).
     eexists; mauto 2.
   Qed.
 
-  Next Obligation. (* nbe_ty_order G {{{ B[Id,,N'] }}} *)
+  Next Obligation. (* nbe_ty_order Γ {{{ B[Id,,N'] }}} *)
     simplify_nbe_order.
     progressive_inversion.
     resolve_alg_sound.
-    assert {{ ⊢ G, ^(A : exp) }} by mauto 2.
+    assert {{ ⊢ Γ, ^(A : exp) }} by mauto 2.
     resolve_alg_sound.
     eexists; mauto 3.
   Qed.
 
-  Next Obligation. (* {{ G ⊢a M' N' ⟹ B' }} /\ (exists i, {{ G ⊢a B' ⟹ Sort@i }}) *)
+  Next Obligation. (* {{ Γ ⊢a M' N' ⟹ B' }} /\ (exists i, {{ Γ ⊢a B' ⟹ Sort@i }}) *)
     progressive_inversion.
     split; [mautosolve 3 |].
     resolve_alg_sound.
-    assert {{ ⊢ G, ^(A : exp) }} by mauto 2.
+    assert {{ ⊢ Γ, ^(A : exp) }} by mauto 2.
     resolve_alg_sound.
-    assert {{ G ⊢s Id,,N' : G, ^(A : exp) }} by mauto 2.
-    assert {{ G ⊢ B[Id,,N'] : ^n{{{ Sort@j }}} }} by mauto 2.
-    assert {{ G ⊢ B[Id,,N'] ≈ B' : Sort@j }} by mauto 2 using soundness_ty'.
+    assert {{ Γ ⊢s Id,,N' : Γ, ^(A : exp) }} by mauto 2.
+    assert {{ Γ ⊢ B[Id,,N'] : ^n{{{ Sort@j }}} }} by mauto 2.
+    assert {{ Γ ⊢ B[Id,,N'] ≈ B' : Sort@j }} by mauto 2 using soundness_ty'.
     assert (user_exp B') by trivial using user_exp_nf.
-    assert (exists k, {{ G ⊢a B' ⟹ Sort@k }} /\ k <= j) as [? []] by (gen_presups; mauto 2).
+    assert (exists k, {{ Γ ⊢a B' ⟹ Sort@k }} /\ k <= j) as [? []] by (gen_presups; mauto 2).
     eexists; eauto 2.
   Qed.
 
-  Next Obligation. (* exists i : nat, {{ G ⊢ B'[Id,,M1'] : Sort@i }} *)
+  Next Obligation. (* exists i : nat, {{ Γ ⊢ B'[Id,,M1'] : Sort@i }} *)
     progressive_inversion.
     resolve_alg_sound.
-    assert {{ ⊢ G, A' }} by mauto 2.
+    assert {{ ⊢ Γ, A' }} by mauto 2.
     resolve_alg_sound.
     eexists; mauto 2.
     eapply wf_conv'; [eapply wf_exp_sub |]; mauto 3.
   Qed.
 
-  Next Obligation. (* nbe_ty_order {{{ G, A' }}} B' *)
+  Next Obligation. (* nbe_ty_order {{{ Γ, A' }}} B' *)
     progressive_inversion.
     resolve_alg_sound.
     simplify_nbe_order.
-    assert {{ ⊢ G, A' }} by mauto 2.
+    assert {{ ⊢ Γ, A' }} by mauto 2.
     resolve_alg_sound.
     eauto.
   Qed.
 
-  Next Obligation. (* {{ G ⊢a ⟨ M1' : A'; M2' : B' ⟩ ⟹ Σ A'' B'' }} /\ (exists i0 : nat, {{ G ⊢a Σ A'' B'' ⟹ Sort@i0 }}) *)
+  Next Obligation. (* {{ Γ ⊢a ⟨ M1' : A'; M2' : B' ⟩ ⟹ Σ A'' B'' }} /\ (exists i0 : nat, {{ Γ ⊢a Σ A'' B'' ⟹ Sort@i0 }}) *)
     progressive_inversion.
     split; [mautosolve 3 |].
     resolve_alg_sound.
-    assert {{ ⊢ G, A' }} by mauto 2.
+    assert {{ ⊢ Γ, A' }} by mauto 2.
     resolve_alg_sound.
-    assert {{ G ⊢ A' ≈ A'' : Sort@i }} by mauto 2 using soundness_ty'.
-    assert {{ G ⊢ A'' : Sort@i }} by (gen_presups; mauto 2).
-    assert {{ G , A' ⊢ B' ≈ B'' : Sort@j }} by mauto 2 using soundness_ty'.
-    assert {{ G , A' ⊢ B'' : Sort@j }} by (gen_presups; mauto 2).
-    assert {{ G , ^(A'':typ) ⊢ B'' : Sort@j }} by (eapply @ctxeq_exp with (Γ:={{{G, A'}}}); mauto 3).
-    assert {{ G ⊢ Σ A'' B'' : Sort@(max i j) }} by mauto 2.
+    assert {{ Γ ⊢ A' ≈ A'' : Sort@i }} by mauto 2 using soundness_ty'.
+    assert {{ Γ ⊢ A'' : Sort@i }} by (gen_presups; mauto 2).
+    assert {{ Γ , A' ⊢ B' ≈ B'' : Sort@j }} by mauto 2 using soundness_ty'.
+    assert {{ Γ , A' ⊢ B'' : Sort@j }} by (gen_presups; mauto 2).
+    assert {{ Γ , ^(A'':typ) ⊢ B'' : Sort@j }} by (eapply @ctxeq_exp with (Γ:={{{Γ, A'}}}); mauto 3).
+    assert {{ Γ ⊢ Σ A'' B'' : Sort@(max i j) }} by mauto 2.
     assert (user_exp n{{{ Σ A'' B'' }}}) by trivial using user_exp_nf.
     eapply alg_type_infer_typ_complete in H57; mauto 3.
     destruct_all. mauto 3.
   Qed.
 
-  Next Obligation. (* {{ G ⊢a fst M' ⟹ A' }} /\ (exists i : nat, {{ G ⊢a A' ⟹ Sort@i }}) *)
+  Next Obligation. (* {{ Γ ⊢a fst M' ⟹ A' }} /\ (exists i : nat, {{ Γ ⊢a A' ⟹ Sort@i }}) *)
     progressive_inversion.
     split; [mautosolve 3 |].
     resolve_alg_sound.
@@ -470,118 +421,118 @@ Section type_check.
     mauto.
   Qed.
 
-  Next Obligation. (* nbe_ty_order G {{{ B[Id,,fst M'] }}} *)
+  Next Obligation. (* nbe_ty_order Γ {{{ B[Id,,fst M'] }}} *)
     progressive_inversion.
     resolve_alg_sound.
     simplify_nbe_order.
-    assert {{ G ⊢ fst M' : A' }} by mauto 2.
-    assert {{ ⊢ G, ^(A':typ) }} by mauto 2.
+    assert {{ Γ ⊢ fst M' : A' }} by mauto 2.
+    assert {{ ⊢ Γ, ^(A':typ) }} by mauto 2.
     resolve_alg_sound.
     eexists.
     eapply wf_conv'; [eapply wf_exp_sub |]; mauto 3.
   Qed.
 
-  Next Obligation.   (* {{ G ⊢a snd M' ⟹ B' }} /\ (exists i : nat, {{ G ⊢a B' ⟹ Sort@i0 }}) *)
+  Next Obligation.   (* {{ Γ ⊢a snd M' ⟹ B' }} /\ (exists i : nat, {{ Γ ⊢a B' ⟹ Sort@i0 }}) *)
     progressive_inversion.
     split; [mautosolve 3 |].
     resolve_alg_sound.
     mauto.
-    assert {{ G ⊢ fst M' : A' }} by mauto 2.
-    assert {{ ⊢ G, ^(A':typ) }} by mauto 2.
+    assert {{ Γ ⊢ fst M' : A' }} by mauto 2.
+    assert {{ ⊢ Γ, ^(A':typ) }} by mauto 2.
     apply wf_sigma_inversion' in H12.
     destruct_all.
-    assert {{ G ⊢ B[Id,,fst M'] ≈ B' : Sort@(max i j) }} by (eapply soundness_ty'; mauto 3).
+    assert {{ Γ ⊢ B[Id,,fst M'] ≈ B' : Sort@(max i j) }} by (eapply soundness_ty'; mauto 3).
     gen_presups.
     assert (user_exp B') by trivial using user_exp_nf.
     eapply alg_type_infer_typ_complete in H18; mauto 3.
     destruct_all. mauto 3.
   Qed.
 
-  Next Obligation. (* {{ G ⊢a refl A' M' ⟹ Eq A'' M'' M'' }} /\ (exists i0 : nat, {{ G ⊢a Eq A'' M'' M'' ⟹ Sort@i0 }}) *)
+  Next Obligation. (* {{ Γ ⊢a refl A' M' ⟹ Eq A'' M'' M'' }} /\ (exists i0 : nat, {{ Γ ⊢a Eq A'' M'' M'' ⟹ Sort@i0 }}) *)
     split; [mautosolve 3 |].
     resolve_alg_sound.
-    assert {{ G ⊢ A' ≈ A'' : Sort@i }} by eauto 2 using soundness_ty'.
-    assert {{ G ⊢ A' ≈ A'' : Sort@i }} by eauto 2 using soundness_ty'.
-    assert {{ G ⊢ M' ≈ M'' : A' }} by eauto 2 using soundness'.
-    assert {{ G ⊢ M' ≈ M'' : A'' }} by mauto 2.
-    assert {{ G ⊢ Eq A'' M'' M'' : Sort@i }} by (gen_presups; mauto 2).
+    assert {{ Γ ⊢ A' ≈ A'' : Sort@i }} by eauto 2 using soundness_ty'.
+    assert {{ Γ ⊢ A' ≈ A'' : Sort@i }} by eauto 2 using soundness_ty'.
+    assert {{ Γ ⊢ M' ≈ M'' : A' }} by eauto 2 using soundness'.
+    assert {{ Γ ⊢ M' ≈ M'' : A'' }} by mauto 2.
+    assert {{ Γ ⊢ Eq A'' M'' M'' : Sort@i }} by (gen_presups; mauto 2).
     assert (user_exp n{{{ Eq A'' M'' M'' }}}) by trivial using user_exp_nf.
-    assert (exists k, {{ G ⊢a Eq A'' M'' M'' ⟹ Sort@k }} /\ k <= i) as [? []] by (gen_presups; mauto 2).
+    assert (exists k, {{ Γ ⊢a Eq A'' M'' M'' ⟹ Sort@k }} /\ k <= i) as [? []] by (gen_presups; mauto 2).
     eexists; eauto 2.
   Qed.
 
-  Next Obligation. (* {{ ⊢ G, A', A'[Wk], Eq A'[Wk∘Wk] #1 #0 }} *)
+  Next Obligation. (* {{ ⊢ Γ, A', A'[Wk], Eq A'[Wk∘Wk] #1 #0 }} *)
     resolve_alg_sound.
-    assert {{ G, A' ⊢s Wk : G }} by mauto 3.
-    assert {{ G, A' ⊢ A'[Wk] : Sort@i }} by mauto 2.
-    assert {{ ⊢ G, A', A'[Wk] }} by mauto 3.
-    assert {{ G, A', A'[Wk] ⊢ Eq A'[Wk∘Wk] #1 #0 : Sort@i }} by mauto 2.
+    assert {{ Γ, A' ⊢s Wk : Γ }} by mauto 3.
+    assert {{ Γ, A' ⊢ A'[Wk] : Sort@i }} by mauto 2.
+    assert {{ ⊢ Γ, A', A'[Wk] }} by mauto 3.
+    assert {{ Γ, A', A'[Wk] ⊢ Eq A'[Wk∘Wk] #1 #0 : Sort@i }} by mauto 2.
     mauto 2.
   Qed.
 
-  Next Obligation. (* exists i0 : nat, {{ G, A' ⊢ B'[Id,,#0,,refl A'[Wk] #0] : Sort@i0 }} *)
+  Next Obligation. (* exists i0 : nat, {{ Γ, A' ⊢ B'[Id,,#0,,refl A'[Wk] #0] : Sort@i0 }} *)
     functional_alg_type_infer_rewrite_clear.
     resolve_alg_sound.
-    assert {{ G, A' ⊢s Wk : G }} by mauto 3.
-    assert {{ G, A' ⊢ A'[Wk] : Sort@i }} by mauto 2.
-    assert {{ ⊢ G, A', A'[Wk] }} by mauto 3.
-    assert {{ G, A', A'[Wk] ⊢ Eq A'[Wk∘Wk] #1 #0 : Sort@i }} by mauto 2.
-    assert {{ G, A', A'[Wk], Eq A'[Wk∘Wk] #1 #0 ⊢ B' : ^n{{{ Sort@j }}} }} by mauto 3 using alg_type_infer_sound.
-    pose proof (@glu_rel_eq_eqrec_synprop_gen_A G {{{ Id }}} _ _ A' ltac:(mauto 2) ltac:(eassumption)).
+    assert {{ Γ, A' ⊢s Wk : Γ }} by mauto 3.
+    assert {{ Γ, A' ⊢ A'[Wk] : Sort@i }} by mauto 2.
+    assert {{ ⊢ Γ, A', A'[Wk] }} by mauto 3.
+    assert {{ Γ, A', A'[Wk] ⊢ Eq A'[Wk∘Wk] #1 #0 : Sort@i }} by mauto 2.
+    assert {{ Γ, A', A'[Wk], Eq A'[Wk∘Wk] #1 #0 ⊢ B' : ^n{{{ Sort@j }}} }} by mauto 3 using alg_type_infer_sound.
+    pose proof (@glu_rel_eq_eqrec_synprop_gen_A Γ {{{ Id }}} _ _ A' ltac:(mauto 2) ltac:(eassumption)).
     destruct_all.
-    assert {{ G, A' ⊢ B'[Id,,#0,,refl A'[Wk] #0] : Sort@j }} by mauto 2.
+    assert {{ Γ, A' ⊢ B'[Id,,#0,,refl A'[Wk] #0] : Sort@j }} by mauto 2.
     eauto.
   Qed.
 
-  Next Obligation. (* nbe_ty_order G {{{ B'[Id,,M1',,M2',,N'] }}} *)
+  Next Obligation. (* nbe_ty_order Γ {{{ B'[Id,,M1',,M2',,N'] }}} *)
     simplify_nbe_order.
     resolve_alg_sound.
-    assert {{ G ⊢ Eq A' M1' M2' : Sort@i }} by mauto 2.
+    assert {{ Γ ⊢ Eq A' M1' M2' : Sort@i }} by mauto 2.
     resolve_alg_sound.
-    assert {{ G, A' ⊢s Wk : G }} by mauto 3.
-    assert {{ G, A' ⊢ A'[Wk] : Sort@i }} by mauto 2.
-    assert {{ ⊢ G, A', A'[Wk] }} by mauto 3.
-    assert {{ G, A', A'[Wk] ⊢ Eq A'[Wk∘Wk] #1 #0 : Sort@i }} by mauto 2.
-    assert {{ G, A', A'[Wk], Eq A'[Wk∘Wk] #1 #0 ⊢ B' : ^n{{{ Sort@j }}} }} by mauto 3 using alg_type_infer_sound.
-    assert {{ G ⊢s Id,,M1',,M2',,N' : G, A', A'[Wk], Eq A'[Wk∘Wk] #1 #0 }} by mauto 2.
+    assert {{ Γ, A' ⊢s Wk : Γ }} by mauto 3.
+    assert {{ Γ, A' ⊢ A'[Wk] : Sort@i }} by mauto 2.
+    assert {{ ⊢ Γ, A', A'[Wk] }} by mauto 3.
+    assert {{ Γ, A', A'[Wk] ⊢ Eq A'[Wk∘Wk] #1 #0 : Sort@i }} by mauto 2.
+    assert {{ Γ, A', A'[Wk], Eq A'[Wk∘Wk] #1 #0 ⊢ B' : ^n{{{ Sort@j }}} }} by mauto 3 using alg_type_infer_sound.
+    assert {{ Γ ⊢s Id,,M1',,M2',,N' : Γ, A', A'[Wk], Eq A'[Wk∘Wk] #1 #0 }} by mauto 2.
     eexists; mauto 2.
   Qed.
 
-  Next Obligation. (* {{ G ⊢a eqrec N' as Eq A' M1' M2' return B' | refl -> BR' end ⟹ B'' }} /\ (exists i0 : nat, {{ G ⊢a B'' ⟹ Sort@i0 }}) *)
+  Next Obligation. (* {{ Γ ⊢a eqrec N' as Eq A' M1' M2' return B' | refl -> BR' end ⟹ B'' }} /\ (exists i0 : nat, {{ Γ ⊢a B'' ⟹ Sort@i0 }}) *)
     split; [mautosolve 3 |].
     resolve_alg_sound.
-    assert {{ G ⊢ Eq A' M1' M2' : Sort@i }} by mauto 2.
+    assert {{ Γ ⊢ Eq A' M1' M2' : Sort@i }} by mauto 2.
     resolve_alg_sound.
-    assert {{ G, A' ⊢s Wk : G }} by mauto 3.
-    assert {{ G, A' ⊢ A'[Wk] : Sort@i }} by mauto 2.
-    assert {{ ⊢ G, A', A'[Wk] }} by mauto 3.
-    assert {{ G, A', A'[Wk] ⊢ Eq A'[Wk∘Wk] #1 #0 : Sort@i }} by mauto 2.
-    assert {{ G, A', A'[Wk], Eq A'[Wk∘Wk] #1 #0 ⊢ B' : ^n{{{ Sort@j }}} }} by mauto 3 using alg_type_infer_sound.
-    assert {{ G ⊢s Id,,M1',,M2',,N' : G, A', A'[Wk], Eq A'[Wk∘Wk] #1 #0 }} by mauto 2.
-    assert {{ G ⊢ B'[Id,,M1',,M2',,N'] : Sort@j }} by mauto 2.
-    assert {{ G ⊢ B'[Id,,M1',,M2',,N'] ≈ B'' : Sort@j }} by eauto 2 using soundness_ty'.
+    assert {{ Γ, A' ⊢s Wk : Γ }} by mauto 3.
+    assert {{ Γ, A' ⊢ A'[Wk] : Sort@i }} by mauto 2.
+    assert {{ ⊢ Γ, A', A'[Wk] }} by mauto 3.
+    assert {{ Γ, A', A'[Wk] ⊢ Eq A'[Wk∘Wk] #1 #0 : Sort@i }} by mauto 2.
+    assert {{ Γ, A', A'[Wk], Eq A'[Wk∘Wk] #1 #0 ⊢ B' : ^n{{{ Sort@j }}} }} by mauto 3 using alg_type_infer_sound.
+    assert {{ Γ ⊢s Id,,M1',,M2',,N' : Γ, A', A'[Wk], Eq A'[Wk∘Wk] #1 #0 }} by mauto 2.
+    assert {{ Γ ⊢ B'[Id,,M1',,M2',,N'] : Sort@j }} by mauto 2.
+    assert {{ Γ ⊢ B'[Id,,M1',,M2',,N'] ≈ B'' : Sort@j }} by eauto 2 using soundness_ty'.
     assert (user_exp B'') by eauto 2 using user_exp_nf.
-    assert (exists k, {{ G ⊢a B'' ⟹ Sort@k }} /\ k <= j) as [? []] by (gen_presups; mauto 2).
+    assert (exists k, {{ Γ ⊢a B'' ⟹ Sort@k }} /\ k <= j) as [? []] by (gen_presups; mauto 2).
     eexists; eauto.
   Qed.
 
-  Final Obligation. (* {{ G ⊢a #x ⟹ A' }} /\ (exists i, {{ G ⊢a A' ⟹ Sort@i }}) *)
+  Final Obligation. (* {{ Γ ⊢a #x ⟹ A' }} /\ (exists i, {{ Γ ⊢a A' ⟹ Sort@i }}) *)
     split; [mautosolve 3 |].
-    assert (exists i, {{ G ⊢ A : Sort@i }}) as [i] by mauto 2.
+    assert (exists i, {{ Γ ⊢ A : Sort@i }}) as [i] by mauto 2.
     resolve_alg_sound.
-    assert {{ G ⊢ A ≈ A' : Sort@i }} by eauto 2 using soundness_ty'.
+    assert {{ Γ ⊢ A ≈ A' : Sort@i }} by eauto 2 using soundness_ty'.
     assert (user_exp A') by trivial using user_exp_nf.
-    assert (exists j, {{ G ⊢a A' ⟹ Sort@j }} /\ j <= i) as [? []] by (gen_presups; mauto 2).
+    assert (exists j, {{ Γ ⊢a A' ⟹ Sort@j }} /\ j <= i) as [? []] by (gen_presups; mauto 2).
     eexists; eauto 2.
   Qed.
 
   Extraction Inline type_check_functional type_infer_functional.
 
-  Lemma type_infer_order_soundness : forall G M A,
-      {{ G ⊢a M ⟹ A }} ->
+  Lemma type_infer_order_soundness : forall Γ M A,
+      {{ Γ ⊢a M ⟹ A }} ->
       type_infer_order M
-  with type_check_order_soundness : forall G M A,
-      {{ G ⊢a M ⟸ A }} ->
+  with type_check_order_soundness : forall Γ M A,
+      {{ Γ ⊢a M ⟸ A }} ->
       type_check_order M.
   Proof.
     - clear type_infer_order_soundness.
@@ -598,9 +549,9 @@ End type_check.
 #[local]
 Hint Resolve type_check_order_soundness type_infer_order_soundness : mcpts.
 
-Lemma type_check_complete' : forall G M A (HA : exists i, {{ G ⊢ A : Sort@i }}),
-    {{ G ⊢a M ⟸ A }} ->
-    exists H H', type_check G A HA M H = left H'.
+Lemma type_check_complete' : forall Γ M A (HA : exists i, {{ Γ ⊢ A : Sort@i }}),
+    {{ Γ ⊢a M ⟸ A }} ->
+    exists H H', type_check Γ A HA M H = left H'.
 Proof.
   intros ? ? ? [] ?.
   assert (Horder : type_check_order M) by mauto.
@@ -608,14 +559,14 @@ Proof.
   dec_complete.
 Qed.
 
-Lemma type_infer_complete : forall G M A (HG : {{ ⊢ G }}),
-    {{ G ⊢a M ⟹ A }} ->
-    exists H H', type_infer G HG M H = inleft (exist _ A H').
+Lemma type_infer_complete : forall Γ M A (HΓ : {{ ⊢ Γ }}),
+    {{ Γ ⊢a M ⟹ A }} ->
+    exists H H', type_infer Γ HΓ M H = inleft (exist _ A H').
 Proof.
   intros.
   assert (Horder : type_infer_order M) by mauto.
   exists Horder.
-  destruct (type_infer G HG M Horder) as [[? []] |].
+  destruct (type_infer Γ HΓ M Horder) as [[? []] |].
   - functional_alg_type_infer_rewrite_clear.
     eexists; reflexivity.
   - contradict H; intuition.
